\subsubsection{Mechanische Leistung} 
\begin{minipage}{0.45\textwidth} 
\mainformular{$ P = \frac{W}{t} $} 
\end{minipage} 
\begin{minipage}{0.45\textwidth} 
 
\legende{}\end{minipage} 
 
$ P = \frac{W}{t} $ - $ W = P\cdot t $ - $ t = \frac{W}{P} $ - \\ 
 
\subsubsection{Wirkungsgrad} 
\begin{minipage}{0.45\textwidth} 
\mainformular{$ \eta  = \frac{P_{2} }{P_{1} } $} 
\end{minipage} 
\begin{minipage}{0.45\textwidth} 
 
\legende{}\end{minipage} 
 
$ \eta  = \frac{P_{2} }{P_{1} } $ - $ P_{1}  = \frac{p_{2} }{\eta } $ - $ P_{2}  = \eta \cdot P_{1} $ - \\ 
 
\subsubsection{Beschleunigungsarbeit - kinetische Energie} 
\begin{minipage}{0.45\textwidth} 
\mainformular{$ W = \frac{1}{2}\cdot m\cdot v^{2} $} 
\end{minipage} 
\begin{minipage}{0.45\textwidth} 
 
\legende{}\end{minipage} 
 
$ W = \frac{1}{2}\cdot m\cdot v^{2} $ - $ m = \frac{2\cdot W}{ v^{2} } $ - $ v = \sqrt{\frac{2\cdot W}{ m}} $ - \\ 
 
\subsubsection{Spannarbeit-Spannenergie} 
\begin{minipage}{0.45\textwidth} 
\mainformular{$ W =\frac{1}{2}\cdot D\cdot s^{2} $} 
\end{minipage} 
\begin{minipage}{0.45\textwidth} 
 
\legende{}\end{minipage} 
 
$ W =\frac{1}{2}\cdot D\cdot s^{2} $ - $ s = \sqrt{\frac{2\cdot W}{ D}} $ - $ D =\frac{2\cdot W}{s^{2} } $ - \\ 
 
\subsubsection{Hubarbeit - Potentielle Energie} 
\begin{minipage}{0.45\textwidth} 
\mainformular{$ W = F_{G} \cdot h $} 
\end{minipage} 
\begin{minipage}{0.45\textwidth} 
 
\legende{}\end{minipage} 
 
$ W = F_{G} \cdot h $ - $ F_{G}  = \frac{W}{h} $ - $ h = \frac{W}{F_{G} } $ - \\ 
 
\subsubsection{Mechanische Arbeit} 
\begin{minipage}{0.45\textwidth} 
\mainformular{$ W = F\cdot s $} 
\end{minipage} 
\begin{minipage}{0.45\textwidth} 
 
\legende{}\end{minipage} 
 
$ W = F\cdot s $ - $ F = \frac{W}{s} $ - $ s = \frac{W}{F} $ - \\ 
 
\subsubsection{Impuls} 
\begin{minipage}{0.45\textwidth} 
\mainformular{$ p = m\cdot v $} 
\end{minipage} 
\begin{minipage}{0.45\textwidth} 
 
\legende{}\end{minipage} 
 
$ p = m\cdot v $ - $ m = \frac{p}{v} $ - $ v = \frac{p}{m} $ - \\ 
 
\subsubsection{Gravitationsgesetz} 
\begin{minipage}{0.45\textwidth} 
\mainformular{$ F = G \cdot  \frac{m_{1} \cdot m_{2} }{  r^{2} } $} 
\end{minipage} 
\begin{minipage}{0.45\textwidth} 
 
\legende{}\end{minipage} 
 
$ F = G \cdot  \frac{m_{1} \cdot m_{2} }{  r^{2} } $ - $ r = \sqrt{\frac{G\cdot m_{1} \cdot m_{2} }{   F}} $ - $ m_{1}  =  \frac{F\cdot r^{2} }{G\cdot m_{2} } $ - $ m_{2}  =  \frac{F\cdot r^{2} }{G\cdot m_{1} } $ - \\ 
 
\subsubsection{Zentralkraft} 
\begin{minipage}{0.45\textwidth} 
\mainformular{$ F_{z}  = m\cdot \omega ^{2} \cdot r $} 
\end{minipage} 
\begin{minipage}{0.45\textwidth} 
 
\legende{}\end{minipage} 
 
$ F_{z}  = m\cdot \omega ^{2} \cdot r $ - $ m = \frac{ F_{z} }{\omega ^{2} \cdot r} $ - $ \omega  = \sqrt{\frac{ F_{z} }{m\cdot r}} $ - $ r = \frac{ F_{z} }{m\cdot \omega ^{2} } $ - \\ 
 
\subsubsection{Schiefe Ebene} 
\begin{minipage}{0.45\textwidth} 
\mainformular{$ F_{H}  = F_{G} \cdot sin \alpha $} 
\end{minipage} 
\begin{minipage}{0.45\textwidth} 
 
\legende{}\end{minipage} 
 
$ F_{H}  = F_{G} \cdot sin \alpha $ - $ F_{G}  = \frac{ F_{H} }{sin \alpha } $ - $ sin \alpha  = \frac{F_{H} }{F_{G} } $ - $ F_{N}  = F_{G} \cdot cos \alpha $ - $ F_{G}  = \frac{ F_{N} }{cos \alpha } $ - $ cos \alpha  = \frac{F_{N} }{F_{G} } $ - \\ 
 
\subsubsection{Kraft} 
\begin{minipage}{0.45\textwidth} 
\mainformular{$ F = m\cdot a $} 
\end{minipage} 
\begin{minipage}{0.45\textwidth} 
 
\legende{}\end{minipage} 
 
$ F = m\cdot a $ - $ m = \frac{F}{a} $ - $ a = \frac{F}{m} $ - \\ 
 
