\subsubsection{Zentralbeschleunigung} 
\begin{minipage}{0.45\textwidth} 
\mainformular{$ a_{z}  = \omega ^{2} \cdot r $} 
\end{minipage} 
\begin{minipage}{0.45\textwidth} 
 
\legende{}\end{minipage} 
 
$ a_{z}  = \omega ^{2} \cdot r $ - $ \omega  = \sqrt{\frac{a_{z} }{r}} $ - $ r = \frac{a_{z} }{\omega } $ - \\ 
 
\subsubsection{Bahngeschwindigkeit} 
\begin{minipage}{0.45\textwidth} 
\mainformular{$ v = \omega \cdot r $} 
\end{minipage} 
\begin{minipage}{0.45\textwidth} 
 
\legende{}\end{minipage} 
 
$ v = \omega \cdot r $ - $ \omega  = \frac{v}{r} $ - $ r = \frac{v}{\omega } $ - \\ 
 
\subsubsection{Winkelgeschwindigkeit} 
\begin{minipage}{0.45\textwidth} 
\mainformular{$ \omega  = 2\cdot \pi \cdot f $} 
\end{minipage} 
\begin{minipage}{0.45\textwidth} 
 
\legende{}\end{minipage} 
 
$ \omega  = 2\cdot \pi \cdot f $ - $ f = \frac{\omega }{2\cdot \pi } $ - $ \omega  = \frac{2\cdot \pi }{ T} $ - $ T = \frac{2\cdot \pi }{ \omega } $ - \\ 
 
\subsubsection{Frequenz-Periodendauer} 
\begin{minipage}{0.45\textwidth} 
\mainformular{$ f = \frac{1}{T} $} 
\end{minipage} 
\begin{minipage}{0.45\textwidth} 
 
\legende{}\end{minipage} 
 
$ f = \frac{1}{T} $ - $ T = \frac{1}{f} $ - $ f = \frac{n}{t} $ - $ t = \frac{n}{f} $ - $ n = f\cdot t $ - \\ 
 
\subsubsection{Schiefer Wurf} 
\begin{minipage}{0.45\textwidth} 
\mainformular{$ x_{w}  = \frac{v_{0} ^{2} \cdot sin(2\cdot \alpha )}{       g} $} 
\end{minipage} 
\begin{minipage}{0.45\textwidth} 
 
\legende{}\end{minipage} 
 
$ x_{w}  = \frac{v_{0} ^{2} \cdot sin(2\cdot \alpha )}{       g} $ - $ t =\frac{v_{0} \cdot sin \alpha }{  g} $ - $ v_{y}  =  v\cdot sin\alpha - g\cdot t $ - $ v= \frac{ v_{y} +g\cdot t}{ sin\alpha } $ - $ v_{x}  = v\cdot  cos\alpha $ - $ v= \frac{ v_{x} }{ cos\alpha } $ - $ v= \sqrt{ v_{x} ^{2} + v_{y} ^{2} } $ - $ v_{x} = \sqrt{ v^{2}  - v_{y} ^{2} } $ - $ v_{y} = \sqrt{ v^{2}  - v_{x} ^{2} } $ - $ v_{y} = tan \alpha \cdot  v_{x} $ - $ tan \alpha = \frac{v_{y} }{v_{x} } $ - $ v_{x} = \frac{v_{y} }{tan \alpha } $ - $ y = x\cdot tan \alpha  - \frac{   g\cdot x^{2} }{2\cdot v^{2} _{0} \cdot cos ^{2}\alpha } $ - $ t =\frac{2\cdot v_{0} \cdot sin \alpha }{ g} $ - \\ 
 
\subsubsection{Waagrechter Wurf} 
\begin{minipage}{0.45\textwidth} 
\mainformular{$ h = \frac{1}{2}\cdot g\cdot t^{2} $} 
\end{minipage} 
\begin{minipage}{0.45\textwidth} 
 
\legende{}\end{minipage} 
 
$ h = \frac{1}{2}\cdot g\cdot t^{2} $ - $ g = \frac{2\cdot h}{t^{2} } $ - $ t = \sqrt{\frac{2\cdot h}{g}} $ - $ s = v\cdot t $ - $ v = \frac{s}{t} $ - \\ 
 
\subsubsection{Senkrechter Wurf nach oben} 
\begin{minipage}{0.45\textwidth} 
\mainformular{$ h = h_{0}  + v_{0} \cdot t - \frac{1}{2}\cdot g\cdot t^{2} $} 
\end{minipage} 
\begin{minipage}{0.45\textwidth} 
 
\legende{}\end{minipage} 
 
$ h = h_{0}  + v_{0} \cdot t - \frac{1}{2}\cdot g\cdot t^{2} $ - $ g = - \frac{2\cdot (h - h_{0}  - v_{0} \cdot t)}{     t^{2} } $ - $ t = \frac{-v_{0}  \pm \sqrt{v_{0} ^{2} +4\cdot 0,5\cdot g\cdot (h_{0}  -h)}}{      -g} $ - $ h_{0}  = h - v_{0} \cdot t + \frac{1}{2}\cdot g\cdot t^{2} $ - $ v = v_{0}  - g\cdot t $ - $ v_{0}  = v + g\cdot t $ - $ t = \frac{v_{0} -v}{  g} $ - $ g = \frac{v_{0}  - v}{  t} $ - \\ 
 
\subsubsection{Freier Fall} 
\begin{minipage}{0.45\textwidth} 
\mainformular{$ h = \frac{1}{2}\cdot g\cdot t^{2} $} 
\end{minipage} 
\begin{minipage}{0.45\textwidth} 
 
\legende{}\end{minipage} 
 
$ h = \frac{1}{2}\cdot g\cdot t^{2} $ - $ g = \frac{2\cdot h}{ t^{2} } $ - $ t = \sqrt{\frac{2\cdot h}{g}} $ - $ v = \sqrt{2\cdot h\cdot g} $ - $ h = \frac{ v^{2} }{2\cdot g} $ - \\ 
 
\subsubsection{Durchschnittsbeschleunigung} 
\begin{minipage}{0.45\textwidth} 
\mainformular{$ a = \frac{v_{1}  - v_{2} }{t_{1}  - t_{2} } $} 
\end{minipage} 
\begin{minipage}{0.45\textwidth} 
 
\legende{}\end{minipage} 
 
$ a = \frac{v_{1}  - v_{2} }{t_{1}  - t_{2} } $ - \\ 
 
\subsubsection{Durchschnittsgeschwindigkeit} 
\begin{minipage}{0.45\textwidth} 
\mainformular{$ v = \frac{x_{1}  - x_{2} }{t_{1}  - t_{2} } $} 
\end{minipage} 
\begin{minipage}{0.45\textwidth} 
 
\legende{}\end{minipage} 
 
$ v = \frac{x_{1}  - x_{2} }{t_{1}  - t_{2} } $ - \\ 
 
\subsubsection{Beschleunigte Bewegung mit Anfangsgeschwindigkeit} 
\begin{minipage}{0.45\textwidth} 
\mainformular{$ v = v_{0}  + a\cdot t $} 
\end{minipage} 
\begin{minipage}{0.45\textwidth} 
 
\legende{}\end{minipage} 
 
$ v = v_{0}  + a\cdot t $ - $ v_{0}  = v - a\cdot t $ - $ t = \frac{v - v_{0} }{a} $ - $ a = \frac{v - v_{0} }{  t} $ - $ s = s_{0}  + v_{0} \cdot t + \frac{1}{2}\cdot a\cdot t^{2} $ - $ a = \frac{2\cdot (s - s_{0}  - v_{0} \cdot t)}{     t^{2} } $ - $ t = \frac{-v_{0}  \pm \sqrt{v_{0} ^{2} -4\cdot 0,5\cdot a\cdot (s_{0}  -s)}}{       a} $ - $ s_{0}  = s - v_{0} \cdot t - \frac{1}{2}\cdot a\cdot t^{2} $ - $ v_{0}  =\frac{s-s_{0} -0,5\cdot a\cdot t^{2} }{    t} $ - $ v  =\sqrt{2\cdot a \cdot s+ v_{0}^2} $ - $ v_{0}  =\sqrt{v^2-2\cdot a \cdot s} $ - \\ 
 
\subsubsection{Geradlinige Bewegung v=konst.} 
\begin{minipage}{0.45\textwidth} 
\mainformular{$ s = v\cdot t $} 
\end{minipage} 
\begin{minipage}{0.45\textwidth} 
 
\legende{}\end{minipage} 
 
$ s = v\cdot t $ - $ v = \frac{s}{t} $ - $ t = \frac{s}{v} $ - \\ 
 
\subsubsection{Beschleunigte Bewegung} 
\begin{minipage}{0.45\textwidth} 
\mainformular{$ v = a\cdot t $} 
\end{minipage} 
\begin{minipage}{0.45\textwidth} 
 
\legende{}\end{minipage} 
 
$ v = a\cdot t $ - $ a = \frac{v}{t} $ - $ t = \frac{v}{a} $ - $ s = \frac{1}{2}\cdot a\cdot t^{2} $ - $ a = \frac{2\cdot s}{t^{2} } $ - $ t = \sqrt{\frac{2\cdot s}{a}} $ - \\ 
 
