\subsubsection{Bewegungsgleichung (harmonische Schwingung)} 
\begin{minipage}{0.45\textwidth} 
\mainformular{$ y = y_{s} \cdot sin(\omega \cdot t+\phi _{0} ) $} 
\end{minipage} 
\begin{minipage}{0.45\textwidth} 
 
\legende{}\end{minipage} 
 
$ y = y_{s} \cdot sin(\omega \cdot t+\phi _{0} ) $ - $ y_{s} = \frac{    y}{sin(\omega \cdot t+\phi _{0} )} $ - $ t = \frac{arcsin(y/y_{s} )-\phi _{0} }{    \omega } $ - \\ 
 
\subsubsection{Periodendauer (harmonische Schwingung)} 
\begin{minipage}{0.45\textwidth} 
\mainformular{$ T = 2\cdot \pi \cdot \sqrt{\frac{m}{D}} $} 
\end{minipage} 
\begin{minipage}{0.45\textwidth} 
 
\legende{}\end{minipage} 
 
$ T = 2\cdot \pi \cdot \sqrt{\frac{m}{D}} $ - $ D= m\cdot \frac{(2\cdot \pi )^{2} }{  T^{2} } $ - $ m= D\cdot \frac{ T^{2} }{(2\cdot \pi )^{2} } $ - \\ 
 
\subsubsection{Lineares Kraftgesetz} 
\begin{minipage}{0.45\textwidth} 
\mainformular{$ F = -D\cdot y $} 
\end{minipage} 
\begin{minipage}{0.45\textwidth} 
 
\legende{}\end{minipage} 
 
$ F = -D\cdot y $ - $ D = \frac{-F}{y} $ - $ y = \frac{-F}{D} $ - \\ 
 
