//subsubsection{Längenausdehnung - Aufgabe:LaengUmdl} 
$ \Delta l = l_{0} \cdot \alpha \cdot \Delta T $\ 
$ l_{0}  = \frac{ \Delta l}{\alpha \cdot \Delta T} $\ 
$ \alpha  = \frac{ \Delta l}{l_{0} \cdot \Delta T} $\ 
$ \Delta T = \frac{ \Delta l}{l_{0} \cdot \alpha } $\ 
//subsubsection{Längenausdehnung} 
$ \Delta l = l_{0} \cdot \alpha \cdot \Delta T $\ 
$ l_{0}  = \frac{ \Delta l}{\alpha \cdot \Delta T} $\ 
$ \alpha  = \frac{ \Delta l}{l_{0} \cdot \Delta T} $\ 
$ \Delta T = \frac{ \Delta l}{l_{0} \cdot \alpha } $\ 
//subsubsection{Volumenausdehnung} 
$ \Delta V = V_{0} \cdot 3\cdot \alpha \cdot \Delta T $\ 
$ V_{0}  = \frac{  \Delta V}{3\cdot \alpha \cdot \Delta T} $\ 
$ \alpha  = \frac{  \Delta V}{V_{0} \cdot \Delta T\cdot 3} $\ 
$ \Delta T = \frac{  \Delta V}{V_{0} \cdot 3\cdot \alpha } $\ 
//subsubsection{Volumenausdehnung - Aufgabe:VolausUmdT} 
$ \Delta V = V_{0} \cdot 3\cdot \alpha \cdot \Delta T $\ 
$ V_{0}  = \frac{  \Delta V}{3\cdot \alpha \cdot \Delta T} $\ 
$ \alpha  = \frac{  \Delta V}{V_{0} \cdot \Delta T\cdot 3} $\ 
$ \Delta T = \frac{  \Delta V}{V_{0} \cdot 3\cdot \alpha } $\ 
//subsubsection{Volumenausdehnung - Aufgabe:VolausUmdV} 
$ \Delta V = V_{0} \cdot 3\cdot \alpha \cdot \Delta T $\ 
$ V_{0}  = \frac{  \Delta V}{3\cdot \alpha \cdot \Delta T} $\ 
$ \alpha  = \frac{  \Delta V}{V_{0} \cdot \Delta T\cdot 3} $\ 
$ \Delta T = \frac{  \Delta V}{V_{0} \cdot 3\cdot \alpha } $\ 
//subsubsection{Flächenausdehnung - Aufgabe:FlaeUmalpha} 
$ \Delta A = A_{0} \cdot 2\cdot \alpha \cdot \Delta T $\ 
$ A_{0}  = \frac{ \Delta A}{2\cdot \alpha \cdot \Delta T} $\ 
$ \alpha  = \frac{ \Delta A}{A_{0} \cdot \Delta T\cdot 2} $\ 
$ \Delta T = \frac{ \Delta A}{A_{0} \cdot 2\cdot \alpha } $\ 
//subsubsection{Flächenausdehnung - Aufgabe:FlaeUmA0} 
$ \Delta A = A_{0} \cdot 2\cdot \alpha \cdot \Delta T $\ 
$ A_{0}  = \frac{ \Delta A}{2\cdot \alpha \cdot \Delta T} $\ 
$ \alpha  = \frac{ \Delta A}{A_{0} \cdot \Delta T\cdot 2} $\ 
$ \Delta T = \frac{ \Delta A}{A_{0} \cdot 2\cdot \alpha } $\ 
//subsubsection{Flächenausdehnung} 
$ \Delta A = A_{0} \cdot 2\cdot \alpha \cdot \Delta T $\ 
$ A_{0}  = \frac{ \Delta A}{2\cdot \alpha \cdot \Delta T} $\ 
$ \alpha  = \frac{ \Delta A}{A_{0} \cdot \Delta T\cdot 2} $\ 
$ \Delta T = \frac{ \Delta A}{A_{0} \cdot 2\cdot \alpha } $\ 
//subsubsection{Längenausdehnung - Aufgabe:LaengUml0} 
$ \Delta l = l_{0} \cdot \alpha \cdot \Delta T $\ 
$ l_{0}  = \frac{ \Delta l}{\alpha \cdot \Delta T} $\ 
$ \alpha  = \frac{ \Delta l}{l_{0} \cdot \Delta T} $\ 
$ \Delta T = \frac{ \Delta l}{l_{0} \cdot \alpha } $\ 
//subsubsection{Längenausdehnung - Aufgabe:LaengUmalpha} 
$ \Delta l = l_{0} \cdot \alpha \cdot \Delta T $\ 
$ l_{0}  = \frac{ \Delta l}{\alpha \cdot \Delta T} $\ 
$ \alpha  = \frac{ \Delta l}{l_{0} \cdot \Delta T} $\ 
$ \Delta T = \frac{ \Delta l}{l_{0} \cdot \alpha } $\ 
//subsubsection{Volumenausdehnung - Aufgabe:VolausUmv0} 
$ \Delta V = V_{0} \cdot 3\cdot \alpha \cdot \Delta T $\ 
$ V_{0}  = \frac{  \Delta V}{3\cdot \alpha \cdot \Delta T} $\ 
$ \alpha  = \frac{  \Delta V}{V_{0} \cdot \Delta T\cdot 3} $\ 
$ \Delta T = \frac{  \Delta V}{V_{0} \cdot 3\cdot \alpha } $\ 
//subsubsection{Volumenausdehnung - Aufgabe:VolausUmalpha} 
$ \Delta V = V_{0} \cdot 3\cdot \alpha \cdot \Delta T $\ 
$ V_{0}  = \frac{  \Delta V}{3\cdot \alpha \cdot \Delta T} $\ 
$ \alpha  = \frac{  \Delta V}{V_{0} \cdot \Delta T\cdot 3} $\ 
$ \Delta T = \frac{  \Delta V}{V_{0} \cdot 3\cdot \alpha } $\ 
//subsubsection{Flächenausdehnung - Aufgabe:FlaeUmdt} 
$ \Delta A = A_{0} \cdot 2\cdot \alpha \cdot \Delta T $\ 
$ A_{0}  = \frac{ \Delta A}{2\cdot \alpha \cdot \Delta T} $\ 
$ \alpha  = \frac{ \Delta A}{A_{0} \cdot \Delta T\cdot 2} $\ 
$ \Delta T = \frac{ \Delta A}{A_{0} \cdot 2\cdot \alpha } $\ 
//subsubsection{Längenausdehnung - Aufgabe:LaengUmdt} 
$ \Delta l = l_{0} \cdot \alpha \cdot \Delta T $\ 
$ l_{0}  = \frac{ \Delta l}{\alpha \cdot \Delta T} $\ 
$ \alpha  = \frac{ \Delta l}{l_{0} \cdot \Delta T} $\ 
$ \Delta T = \frac{ \Delta l}{l_{0} \cdot \alpha } $\ 
//subsubsection{Flächenausdehnung - Aufgabe:FlaeUmdA} 
$ \Delta A = A_{0} \cdot 2\cdot \alpha \cdot \Delta T $\ 
$ A_{0}  = \frac{ \Delta A}{2\cdot \alpha \cdot \Delta T} $\ 
$ \alpha  = \frac{ \Delta A}{A_{0} \cdot \Delta T\cdot 2} $\ 
$ \Delta T = \frac{ \Delta A}{A_{0} \cdot 2\cdot \alpha } $\ 
