\subsubsection{Volumenausdehnung} 
\begin{minipage}{0.45\textwidth} 
$ \Delta V = V_{0} \cdot 3\cdot \alpha \cdot \Delta T $\\ 
$ V_{0}  = \frac{  \Delta V}{3\cdot \alpha \cdot \Delta T} $\\ 
$ \alpha  = \frac{  \Delta V}{V_{0} \cdot \Delta T\cdot 3} $\\ 
$ \Delta T = \frac{  \Delta V}{V_{0} \cdot 3\cdot \alpha } $\\ 
\end{minipage} 
\begin{minipage}{0.45\textwidth} 
 
\end{minipage} 
\subsubsection{Flächenausdehnung} 
\begin{minipage}{0.45\textwidth} 
$ \Delta A = A_{0} \cdot 2\cdot \alpha \cdot \Delta T $\\ 
$ A_{0}  = \frac{ \Delta A}{2\cdot \alpha \cdot \Delta T} $\\ 
$ \alpha  = \frac{ \Delta A}{A_{0} \cdot \Delta T\cdot 2} $\\ 
$ \Delta T = \frac{ \Delta A}{A_{0} \cdot 2\cdot \alpha } $\\ 
\end{minipage} 
\begin{minipage}{0.45\textwidth} 
 
\end{minipage} 
\subsubsection{Längenausdehnung} 
\begin{minipage}{0.45\textwidth} 
$ \Delta l = l_{0} \cdot \alpha \cdot \Delta T $\\ 
$ l_{0}  = \frac{ \Delta l}{\alpha \cdot \Delta T} $\\ 
$ \alpha  = \frac{ \Delta l}{l_{0} \cdot \Delta T} $\\ 
$ \Delta T = \frac{ \Delta l}{l_{0} \cdot \alpha } $\\ 
\end{minipage} 
\begin{minipage}{0.45\textwidth} 
 
\end{minipage} 
